2 lemmas left

src/Assembly.v
@@ -50,7 +50,7 @@ Inductive semantics (p p' : state) : Prop :=
           prog p = prog p' -> mem p = mem p' -> ac p = ac p' ->
           pc p' = addr -> semantics p p'
   | skipnz:read_instr p Skip -> prog p = prog p' -> mem p = mem p' ->
-           ac p = ac p' -> Common.lookup (mem p') (ac p') 0 -> pc p' = pc p + 2 -> semantics p p'
+           ac p = ac p' -> ~ Common.lookup (mem p') (ac p') 0 -> pc p' = pc p + 2 -> semantics p p'
   | skipz: read_instr p Skip -> prog p = prog p' -> mem p = mem p' ->
            ac p = ac p' -> Common.lookup (mem p') (ac p') 0 -> pc p' = pc p + 1 -> semantics p p'.
 End Assembly.
